irfewbrjf

LeanGrow/F/Data/RExprTests/RExprMatch.lean
@@ -23,48 +23,89 @@ def List.assignOrFail [BEq α] (A? : Option (List (Nat × α))) (i : Nat) (val :
       | _ => .none
 
 
+
+def List.get?_tail : Nat → List α → Option (α × List α)
+| 0, x :: l => .some (x, l)
+| n+1, _ :: l => List.get?_tail n l
+| _, [] => .none
+
+
+
 partial def RExpr.MatchAssignLFF (delta : Name → RExpr) (l r : RExpr) : Option (List (Nat × NodeExpr)) :=
-      let rec go (go? : Bool) (Aout : Option (List (Nat × NodeExpr))) (todo : List (RExpr × RExpr)) : Option (List (Nat × NodeExpr)) :=
+      let rec go (go? : Bool) (Aout : Option (List (Nat × NodeExpr))) (todo : List ((RExpr × List RExpr) × (RExpr × List RExpr))) : Option (List (Nat × NodeExpr)) :=
       if go?
       then
             match todo with
             | [] => Aout
             | nx :: L =>
                   match nx with
-                  | (.lnode i .none, .lnode j t) => let Aup := List.assignOrFail Aout i (.ofLNode j t) ; go true Aup L
-                  | (.lnode i .none, .gnode j) => let Aup := List.assignOrFail Aout i (.ofGNode j) ; go true Aup L
-                  | (.lnode i .none, e) => let Aup := List.assignOrFail Aout i (.ofRExpr e) ; go true Aup L
-                  | (.bvar i , .bvar j) => go (i == j) Aout L
-                  | (.sort _, .sort _) => go true Aout L
-                  | (.axm n _, .axm n' _) =>  go (n == n')  Aout L
-                  | (.ctor n _, .ctor n' _) =>  go (n.name == n'.name)  Aout L
-                  | (.indt n _, .indt n' _) =>  go (n.name == n'.name)  Aout L
-                  | (.quo n _, .quo n' _) =>  go (n.name == n'.name) Aout L
-                  | (.deltaDef n _, .deltaDef n' _) =>
+                  -- unify
+                  | ((.lnode i .none, _), (.lnode j t, _)) => let Aup := List.assignOrFail Aout i (.ofLNode j t) ; go true Aup L
+                  | (.lnode i .none, .gnode j, _) => let Aup := List.assignOrFail Aout i (.ofGNode j) ; go true Aup L
+                  | (.lnode i .none, e, _) => let Aup := List.assignOrFail Aout i (.ofRExpr e) ; go true Aup L
+                  -- eq
+                  | (.lit l, .lit l', _) => go (l == l') Aout L
+                  | (.bvar i , .bvar j, _) => go (i == j) Aout L
+                  | (.sort _, .sort _, _) => go true Aout L
+                  | (.axm n _, .axm n' _, _) =>  go (n == n')  Aout L
+                  | (.ctor n _, .ctor n' _, _) =>  go (n.name == n'.name)  Aout L
+                  | (.indt n _, .indt n' _, _) =>  go (n.name == n'.name)  Aout L
+                  | (.quo n _, .quo n' _, _) =>  go (n.name == n'.name) Aout L
+                  -- nabla
+                  | (.deltaFun n l, .lam _ _ (.app more (.bvar 0)) _, ctx) =>
+                        go true Aout ((.deltaFun n l, more, ctx) :: L)
+                  | (.lam _ _ (.app more (.bvar 0)) _, .deltaFun n l, ctx) =>
+                        go true Aout ((more, .deltaFun n l, ctx) :: L)
+                  | (.lam n t b l, .lam _ _ (.app more (.bvar 0)) _, ctx) =>
+                        go true Aout ((.lam n t b l, more, ctx) :: L)
+                  | (.lam _ _ (.app more (.bvar 0)) _, .lam n t b l, ctx) =>
+                        go true Aout ((more, .lam n t b l, ctx) :: L)
+                  -- delta
+                  | (.deltaDef n _, .deltaDef n' _, ctx) =>
                         if n == n'
                         then go true Aout L
-                        else go true Aout ((delta n, delta n'):: L)
-                  | (.deltaDef n _, r) => go true Aout ((delta n, r):: L)
-                  | (r, .deltaDef n _) => go true Aout ((r, delta n):: L)
-                  | (.deltaFun n _, .deltaFun n' _) =>
+                        else go true Aout ((delta n, delta n', ctx):: L)
+                  | (.deltaDef n _, r, ctx) => go true Aout ((delta n, r, ctx):: L)
+                  | (r, .deltaDef n _, ctx) => go true Aout ((r, delta n, ctx):: L)
+                  | (.deltaFun n _, .deltaFun n' _, ctx) =>
                         if n == n'
                         then go true Aout L
-                        else go true Aout ((delta n, delta n'):: L)
-                  | (.deltaFun n _, r) => go true Aout ((delta n, r):: L)
-                  | (r, .deltaFun n _) => go true Aout ((r, delta n):: L)
-                  | (.proof v t, .proof v' t') =>
-                        match go true Aout [(v,v')] with
+                        else go true Aout ((delta n, delta n', ctx):: L)
+                  | (.deltaFun n _, r) => go true Aout ((delta n, r, ctx):: L)
+                  | (r, .deltaFun n _) => go true Aout ((r, delta n, ctx):: L)
+                  -- proof irrelevance
+                  | (.proof v t, .proof v' t', ctx) =>
+                        match go true Aout [(v,v', ctx)] with
                         | .some M => go true (.some M) L
                         | .none =>
-                              match go true Aout [(t,t')] with
+                              match go true Aout [(t,t', ctx)] with
                               | .some M =>  go true (.some M) L
-                  -- todo
-                  | (.app f a, .app f' a') => go true Aout ((f,f') :: (a,a') :: L)
-                  | (.lam _ t b _, .lam _ t' b' _) => go true Aout ((t,t') :: (b,b') :: L)
-                  | (.forallE _ t b _, .forallE _ t' b' _) => go true Aout ((t,t') :: (b,b') :: L)
-                  | (.letE _ t v b _, .letE _ t' v' b' _) => go true Aout ((t,t') :: (v,v') :: (b,b') :: L)
-                  | (.lit l, .lit l') => go (l == l') Aout L
-                  | (.proj t i b, .proj t' i' b') => go ((t == t') && (i == i')) Aout ((b, b') :: L)
+                              -- As can be seen in `Lean.Meta.isDefEqProofIrrel` if the props unify, the proofs are equal
+                              -- and we don't have to track this so as to mention prop irrel thms when reconstructing
+                              | .none => .none
+                  -- regular
+                  | (.app f a, .app f' a', ctx) => go true Aout ((f,f', ctx) :: (a,a', ctx) :: L)
+                  | (.lam _ t b _, .lam _ t' b' _, ctx) => go true Aout ((t,t', ctx) :: (b,b', ctx) :: L)
+                  | (.forallE _ t b _, .forallE _ t' b' _, ctx) => go true Aout ((t,t', ctx) :: (b,b', ctx) :: L)
+                  | (.letE _ t v b _, .letE _ t' v' b' _, ctx) => go true Aout ((t,t', ctx) :: (v,v', ctx) :: (b,b', ctx) :: L)
+                  | (.proj t i b, .proj t' i' b', ctx) => go ((t == t') && (i == i')) Aout ((b, b', ctx) :: L)
+                  -- projection reduction
+                  | (.proj n i (.struc n' f), more, ctx) => go (n == n') Aout ((f.get! i, more, ctx) :: L)
+                  | (more, .proj n i (.struc n' f), ctx) => go (n == n') Aout ((more, f.get! i, ctx) :: L)
+                  -- eta (shouldn't be required if we eta expand in cahce and in query, hence :)
+                  | (.struc n p, .struc n' p') => go (n == n') Aout ((List.zip p (p'.map (fun x => (x, ctx)))) ++ L)
+                  -- beta
+                  | ((.app (.lam _ _ B _) (A), lctx), (more, rctx)) => go true Aout (((B, A :: lctx), (more, rctx)) :: L)
+                  | ((more, lctx), (.app (.lam _ _ B _) (A), rctx)) => go true Aout (((more, lctx), (B, A :: rctx)) :: L)
+                  | ((.bvar i, lctx) (t, rctx)) =>
+                        match List.get?_tail i ltcx with
+                        | .some (b,c) => go true Aout (((b,c),(t,rctx)) :: L)
+                        | _ => .none
+                  -- todo sym and fix ↑
+                  -- no match
                   | (_ , _) => .none
       else .none
       go true (.some []) [(l,r)]
+
+
+#check List.zip
